
\chapter{Grammars}

\section{Context Free Grammars}

\begin{example}
$E' \rightarrow E$;
$E \rightarrow T \text{+} E | T$;
$T \rightarrow F \times T | F$;
$F \rightarrow D | \text{(} E \text{)}$;
$D \rightarrow \text{0} | \text{1} | \dotsm | \text{9}$;
\end{example}

We do a \textit{left factorisation}. 
Each alternative can start with the same thing. 

An expression can start with a term.
A term can start with a factor.


$E' \rightarrow E$;
$E \rightarrow T (\text{+} E | \epsilon)$;
$T \rightarrow F (\times T | \epsilon)$;
$F \rightarrow D | \text{(} E \text{)}$;
$D \rightarrow \text{0} | \text{1} | \dotsm | \text{9}$;

